src/FrameStack/Compatibility.v
@@ -4471,4 +4471,3 @@ Proof.
   intros. apply H in H0. now apply Rrel_exp_compat_closed_reverse.
 Qed.
 
-
