src/FrameStack/Examples.v
@@ -2,34 +2,6 @@ From CoreErlang.FrameStack Require Export CIU.
 
 Import ListNotations.
 
-Ltac scope_solver_step :=
-  match goal with 
-  | |- EXP _ ⊢ _ => constructor; simpl; auto
-  | |- VAL _ ⊢ _ => constructor; simpl; auto
-  | |- RED _ ⊢ _ => constructor; simpl; auto
-  | |- NVAL _ ⊢ _ => constructor; simpl; auto
-  | |- forall i, i < _ -> _ => simpl; intros
-  | [H : ?i < _ |- _] => inv H; simpl in *; auto; try lia
-  | [H : ?i <= _ |- _] => inv H; simpl in *; auto; try lia
-  | [H : EXP ?n1 ⊢ ?e |- EXP ?n2 ⊢ ?e] => try now (eapply (loosen_scope_exp n2 n1 ltac:(lia)) in H)
-  | [H : VAL ?n1 ⊢ ?e |- VAL ?n2 ⊢ ?e] => try now (eapply (loosen_scope_val n2 n1 ltac:(lia)) in H)
-  | [H : NVAL ?n1 ⊢ ?e |- NVAL ?n2 ⊢ ?e] => try now (eapply (loosen_scope_nonval n2 n1 ltac:(lia)) in H)
-  end.
-
-Ltac scope_solver := repeat scope_solver_step; try lia.
-
-Ltac deriv :=
-  match goal with
-  | [H : ?i < length _ |- _] => simpl in *; inv H; auto; try lia
-  | [H : ?i <= length _ |- _] => simpl in *; inv H;  auto; try lia
-  | [H : | _, _ | ↓ |- _] => inv H; try inv_val
-  | [H : | _ :: _, RValSeq _ | _ ↓ |- _] => inv H; try inv_val
-  | [H : | _ :: _, RExc _ | _ ↓ |- _] => inv H; try inv_val
-  | [H : | _, RExp (EExp _) | _ ↓ |- _] => inv H; try inv_val
-  | [H : | _, RExp (VVal _) | _ ↓ |- _] => inv H; try inv_val
-  | [H : | _, RBox | _ ↓ |- _] => inv H; try inv_val
-  end.
-
 Ltac extract_meta_eval H :=
   let r := fresh "r" in
   let k := fresh "k" in
