src/FrameStack/SubstSemantics.v
@@ -33,6 +33,7 @@ Inductive step : FrameStack -> Redex -> FrameStack -> Redex -> Prop :=
 
 (** Cooling: single value *)
 | cool_value v xs:
+  VALCLOSED v -> (* to filter out variables *)
   ⟨ xs, `v ⟩ --> ⟨ xs, RValSeq [v] ⟩
 
 (************************************************)
